Define new type checking function and add some initial definitions for the typechecker.

WebAssembly/Wasm_Checker.thy
@@ -59,7 +59,210 @@ proof (induction "(is@[i])")
     using list_all_conv_same_lab_h[OF Cons(3)]
     by (metis option.distinct(1) same_lab.simps(2) same_lab_h.simps(2))
 qed auto
-    
+
+fun b_e_type_checker :: "t_context \<Rightarrow>  b_e list \<Rightarrow> tf \<Rightarrow> bool"
+and check :: "t_context \<Rightarrow> b_e list \<Rightarrow> c_t \<Rightarrow> c_t option"
+and check_single :: "t_context \<Rightarrow>  b_e \<Rightarrow> c_t \<Rightarrow> c_t option" where
+  check_top:"b_e_type_checker \<C> es (tn _> tm) =
+    (case (check \<C> es (tn, Reach)) of
+      None \<Rightarrow> False
+    | Some ts \<Rightarrow>  c_types_agree ts tm)"
+| check_iter:"check \<C> es ts = (case es of
+                                 [] \<Rightarrow> Some ts
+                               | (e#es) \<Rightarrow> (case (check_single \<C> e ts) of 
+                                              Some ts' \<Rightarrow> check \<C> es ts'))
+                                           "
+  (* num ops *)
+| check_const_num:"check_single \<C> (EConstNum v) ts = type_update ts [] ([T_num (typeof_num v)])"
+| check_const_vec:"check_single \<C> (EConstVec v) ts = type_update ts [] ([T_vec (typeof_vec v)])"
+| check_unop:"check_single \<C> (Unop t op) ts = (if unop_t_num_agree op t
+                                                then type_update ts [T_num t] [T_num t]
+                                                else None)"
+| check_binop:"check_single \<C> (Binop t op) ts = (if binop_t_num_agree op t
+                                                   then type_update ts [(T_num t), (T_num t)] ([T_num t])
+                                                   else None)"
+| check_testop:"check_single \<C> (Testop t _) ts = (if is_int_t_num t
+                                                    then type_update ts [(T_num t)] ([T_num T_i32])
+                                                    else None)"
+| check_relop:"check_single \<C> (Relop t op) ts = (if relop_t_num_agree op t
+                                                   then type_update ts [(T_num t), (T_num t)] ([T_num T_i32])
+                                                   else None)"
+  (* vector ops *)
+| check_unop_vec:"check_single \<C> (Unop_vec op) ts = (type_update ts [(T_vec T_v128)] ([T_vec T_v128]))"
+| check_binop_vec:"check_single \<C> (Binop_vec op) ts = (if binop_vec_wf op
+                                                               then type_update ts [(T_vec T_v128), (T_vec T_v128)] ([T_vec T_v128])
+                                                               else None)"
+| check_ternop_vec:"check_single \<C> (Ternop_vec op) ts = (type_update ts [(T_vec T_v128), (T_vec T_v128), (T_vec T_v128)] ([T_vec T_v128]))"
+| check_test_vec:"check_single \<C> (Test_vec op) ts = (type_update ts [(T_vec T_v128)] ([T_num T_i32]))"
+| check_shift_vec:"check_single \<C> (Shift_vec op) ts = (type_update ts [(T_vec T_v128), (T_num T_i32)] ([T_vec T_v128]))"
+| check_splat_vec:"check_single \<C> (Splat_vec sv) ts = (type_update ts [(T_num (vec_lane_t sv))] ([T_vec T_v128]))"
+| check_extract_vec:"check_single \<C> (Extract_vec sv sx i) ts = (if i < vec_num sv \<and> (sx = U \<or> vec_length sv \<le> 2)
+                                                                 then type_update ts [(T_vec T_v128)] ([T_num (vec_lane_t sv)])
+                                                                 else None)"
+| check_replace_vec:"check_single \<C> (Replace_vec sv i) ts = (if i < vec_num sv
+                                                               then type_update ts [(T_vec T_v128), (T_num (vec_lane_t sv))] ([T_vec T_v128])
+                                                               else None)"
+  \<comment> \<open>\<open>references\<close>\<close>
+| check_null_ref: "check_single \<C> (Null_ref t) ts = type_update ts [] [T_ref t]"
+| check_is_null_ref: "check_single \<C> (Is_null_ref) ts = type_update_is_null_ref ts"
+| check_ref_func: "check_single \<C> (Ref_func j) ts = (if j < length (func_t \<C>) \<and> j \<in> set (refs \<C>) then type_update ts [] [T_ref T_func_ref] else None)"
+(* convert *)
+| check_convert:"check_single \<C> (Cvtop t1 Convert t2 sat_sx) ts = (if (convert_cond t1 t2 sat_sx)
+                                                                     then type_update ts [(T_num t2)] ([T_num t1])
+                                                                     else None)"
+  (* reinterpret *)
+| check_reinterpret:"check_single \<C> (Cvtop t1 Reinterpret t2 sx) ts = (if ((t1 \<noteq> t2) \<and> t_num_length t1 = t_num_length t2 \<and> sx = None)
+                                                                         then type_update ts [(T_num t2)] ([T_num t1])
+                                                                         else None)"
+  (* unreachable, nop, drop, select *)
+| check_unreachable:"check_single \<C> (Unreachable) ts = Some ([], Unreach)"
+| check_nop:"check_single \<C> (Nop) ts = Some ts"
+| check_drop:"check_single \<C> (Drop) ts = type_update_drop ts"
+| check_select:"check_single \<C> (Select t_tag) ts = type_update_select ts t_tag"
+  (* block *)                                 
+| check_block:"check_single \<C> (Block tb es) ts = (case tb_tf_t \<C> tb of
+                                                    Some (tn _> tm) \<Rightarrow>
+                                                      (if (b_e_type_checker (\<C>\<lparr>label := ([tm] @ (label \<C>))\<rparr>) es (tn _> tm))
+                                                        then type_update ts tn tm
+                                                        else None)
+                                                  | None \<Rightarrow> None)"
+  (* loop *)
+| check_loop:"check_single \<C> (Loop tb es) ts = (case tb_tf_t \<C> tb of
+                                                  Some (tn _> tm) \<Rightarrow>
+                                                    (if (b_e_type_checker (\<C>\<lparr>label := ([tn] @ (label \<C>))\<rparr>) es (tn _> tm))
+                                                      then type_update ts tn tm
+                                                      else None)
+                                                | None \<Rightarrow> None)"
+  (* if *)
+| check_if:"check_single \<C> (If tb es1 es2) ts = (case tb_tf_t \<C> tb of
+                                                   Some (tn _> tm) \<Rightarrow> (if (b_e_type_checker (\<C>\<lparr>label := ([tm] @ (label \<C>))\<rparr>) es1 (tn _> tm)
+                                                              \<and> b_e_type_checker (\<C>\<lparr>label := ([tm] @ (label \<C>))\<rparr>) es2 (tn _> tm))
+                                                            then type_update ts (tn@[T_num T_i32]) tm
+                                                            else None)
+                                                 | None => None)"
+  (* br *)
+| check_br:"check_single \<C> (Br i) ts = (if i < length (label \<C>) \<and> (consume ts ((label \<C>)!i)) \<noteq> None
+                                         then (Some ([], Unreach))
+                                         else None)"
+  (* br_if *)
+| check_br_if:"check_single \<C> (Br_if i) ts = (if i < length (label \<C>)
+                                                then type_update ts (((label \<C>)!i @ [T_num T_i32])) (((label \<C>)!i))
+                                                else None)"
+  (* br_table *)
+| check_br_table:"check_single \<C> (Br_table is i) ts = (case (same_lab (is@[i]) (label \<C>)) of
+                                                        None \<Rightarrow> None
+                                                      | Some tls \<Rightarrow>  (if ((consume ts (tls @ [T_num T_i32])) \<noteq> None) then Some ([], Unreach) else None))"
+  (* return *)
+| check_return:"check_single \<C> (Return) ts = (case (return \<C>) of
+                                               None \<Rightarrow> None
+                                             | Some tls \<Rightarrow> (if ((consume ts tls) \<noteq> None) then Some ([], Unreach) else None))"
+  (* call *)
+| check_call:"check_single \<C> (Call i) ts = (if i < length (func_t \<C>)
+                                              then (case ((func_t \<C>)!i) of
+                                                      (tn _> tm) \<Rightarrow> type_update ts tn tm)
+                                              else None)"
+  (* | call_indirect:"\<lbrakk>i < length(types_t \<C>); (types_t \<C>)!i = (t1s _> t2s); ti < length (table \<C>); (table \<C>)!ti = T_tab _  T_func_ref\<rbrakk> \<Longrightarrow> \<C> \<turnstile> [Call_indirect ti i] : (t1s @ [T_num T_i32] _> t2s)" *)
+  (* call_indirect *)
+| check_call_indirect:"check_single \<C> (Call_indirect ti i) ts = (if i < length (types_t \<C>) \<and> ti < length (table \<C>)
+                                                                then
+                                                                  (case ((types_t \<C>)!i, (table \<C>)!ti) of
+                                                                    ((tn _> tm), T_tab _  T_func_ref) \<Rightarrow> type_update ts ((tn@[T_num T_i32])) (tm)
+                                                                  | _ \<Rightarrow> None)
+                                                                else None)"
+  (* get_local *)
+| check_get_local:"check_single \<C> (Get_local i) ts = (if i < length (local \<C>)
+                                                        then type_update ts [] [(local \<C>)!i]
+                                                        else None)"
+  (* set_local *)
+| check_set_local:"check_single \<C> (Set_local i) ts = (if i < length (local \<C>)
+                                                        then type_update ts [(local \<C>)!i] []
+                                                        else None)"
+  (* tee_local *)
+| check_tee_local:"check_single \<C> (Tee_local i) ts = (if i < length (local \<C>)
+                                                       then type_update ts [(local \<C>)!i] [(local \<C>)!i]
+                                                       else None)"
+  (* get_global *)
+| check_get_global:"check_single \<C> (Get_global i) ts = (if i < length (global \<C>)
+                                                         then type_update ts [] [tg_t ((global \<C>)!i)]
+                                                         else None)"
+  (* set_global *)
+| check_set_global:"check_single \<C> (Set_global i) ts = (if i < length (global \<C>) \<and> is_mut (global \<C> ! i)
+                                                         then type_update ts [tg_t ((global \<C>)!i)] []
+                                                         else None)"
+  (* load *)
+| check_load:"check_single \<C> (Load t tp_sx a off) ts = (if length (memory \<C>) \<ge> 1 \<and> load_store_t_bounds a (option_projl tp_sx) t
+                                                         then type_update ts [T_num T_i32] [T_num t]
+                                                         else None)"
+  (* store *)
+| check_store:"check_single \<C> (Store t tp a off) ts = (if length (memory \<C>) \<ge> 1 \<and> load_store_t_bounds a tp t
+                                                         then type_update ts [T_num T_i32, T_num t] []
+                                                         else None)"
+  (* load_vec *)
+| check_load_vec:"check_single \<C> (Load_vec lv a off) ts = (if length (memory \<C>) \<ge> 1 \<and> load_vec_t_bounds lv a
+                                                             then type_update ts [T_num T_i32] [T_vec T_v128]
+                                                             else None)"
+  (* load_lane_vec *)
+| check_load_lane_vec:"check_single \<C> (Load_lane_vec svi i a off) ts = (if length (memory \<C>) \<ge> 1 \<and> (i < vec_i_num svi \<and> 2^a \<le> (vec_i_length svi))
+                                                                         then type_update ts [T_num T_i32, T_vec T_v128] [T_vec T_v128]
+                                                                         else None)"
+  (* store_vec *)
+| check_store_vec:"check_single \<C> (Store_vec sv a off) ts = (if length (memory \<C>) \<ge> 1 \<and> store_vec_t_bounds sv a
+                                                               then type_update ts [T_num T_i32, T_vec T_v128]  []
+                                                               else None)"
+  (* current_memory *)
+| check_current_memory:"check_single \<C> Current_memory ts = (if length (memory \<C>) \<ge> 1
+                                                             then type_update ts []  [T_num T_i32]
+                                                             else None)"
+  (* grow_memory *)
+| check_grow_memory:"check_single \<C> Grow_memory ts = (if length (memory \<C>) \<ge> 1
+                                                        then type_update ts [T_num T_i32] [T_num T_i32]
+                                                        else None)"
+  (* memory_init *)
+| check_memory_init: "check_single \<C> (Memory_init i) ts = (if length (memory \<C>) \<ge> 1 \<and> i < length (data \<C>)
+                                                        then type_update ts [T_num T_i32, T_num T_i32, T_num T_i32] []
+                                                        else None)"
+  (* memory_copy *)
+| check_memory_copy:"check_single \<C> Memory_copy ts = (if length (memory \<C>) \<ge> 1
+                                                        then type_update ts [T_num T_i32, T_num T_i32, T_num T_i32] []
+                                                        else None)"
+  (* memory_fill *)
+| check_memory_fill:"check_single \<C> Memory_fill ts = (if length (memory \<C>) \<ge> 1
+                                                        then type_update ts [T_num T_i32, T_num T_i32, T_num T_i32] []
+                                                        else None)"
+  (* table set *)
+| check_table_set:"check_single \<C> (Table_set ti) ts = (if ti < length (table \<C>)
+                                                            then type_update ts [T_num T_i32, T_ref (tab_t_reftype (table \<C>!ti))] []
+                                                            else None)"
+  (* table get *)
+| check_table_get:"check_single \<C> (Table_get ti) ts = (if ti < length (table \<C>)
+                                                            then type_update ts [T_num T_i32] [T_ref (tab_t_reftype (table \<C>!ti))]
+                                                            else None)"
+  (* table size *)
+| check_table_size:"check_single \<C> (Table_size ti) ts = (if ti < length (table \<C>)
+                                                            then type_update ts [] [T_num T_i32]
+                                                            else None)"
+  (* table grow *)
+| check_table_grow:"check_single \<C> (Table_grow ti) ts = (if ti < length (table \<C>)
+                                                            then type_update ts [T_ref (tab_t_reftype (table \<C>!ti)), T_num T_i32] []
+                                                            else None)"
+| check_table_init:"check_single \<C> (Table_init x y) ts = (if x < length (table \<C>) \<and> y < length (elem \<C>) \<and> tab_t_reftype (table \<C>!x) = elem \<C>!y
+                                                            then type_update ts [T_num T_i32, T_num T_i32, T_num T_i32] []
+                                                            else None)"
+  (* table_init *)
+| check_table_copy:"check_single \<C> (Table_copy x y) ts = (if x < length (table \<C>) \<and> y < length (table \<C>) \<and> tab_t_reftype (table \<C>!x) = elem \<C>!y
+                                                            then type_update ts [T_num T_i32, T_num T_i32, T_num T_i32] []
+                                                            else None)"
+  (* table_fill *)
+| check_table_fill:"check_single \<C> (Table_fill x) ts = (if x < length (table \<C>)
+                                                            then type_update ts [T_num T_i32, T_ref (tab_t_reftype (table \<C>!x)), T_num T_i32] []
+                                                            else None)"
+  (* elem_drop *)
+| check_elem_drop:"check_single \<C> (Elem_drop x) ts = (if x < length (elem \<C>) then type_update ts [] [] else None)"
+  (* data_drop *)
+| check_data_drop:"check_single \<C> (Data_drop x) ts = (if x < length (data \<C>) then type_update ts [] [] else None)"
+
+
+(*
 fun b_e_type_checker :: "t_context \<Rightarrow>  b_e list \<Rightarrow> tf \<Rightarrow> bool"
 and check :: "t_context \<Rightarrow> b_e list \<Rightarrow> checker_type \<Rightarrow> checker_type"
 and check_single :: "t_context \<Rightarrow>  b_e \<Rightarrow> checker_type \<Rightarrow> checker_type" where
@@ -215,5 +418,5 @@ foldl_Cons: "foldl f a (x # xs) = foldl f (f a x) xs"
 | check_grow_memory:"check_single \<C> Grow_memory ts = (if length (memory \<C>) \<ge> 1
                                                         then type_update ts [TSome (T_num T_i32)] (Type [T_num T_i32])
                                                         else Bot)"
-
+*)
 end
